IronFleetDefault/ironfleet/src/Dafny/Distributed/Protocol/CausalMesh/proof/monotonic_read.dfy
@@ -4,7 +4,7 @@ include "packet_sending.dfy"
 include "message_read_reply.dfy"
 include "../../../Common/Collections/Seqs.s.dfy"
 
-module CausalMesh_Proof_CausalRead_i {
+module CausalMesh_Proof_Monotonic_Read_i {
 import opened CausalMesh_Cache_i
 import opened CausalMesh_Message_i
 import opened CausalMesh_Types_i
@@ -126,19 +126,6 @@ predicate AllReadReplyHasCorrspondingReadWithSmallOrEqVCForSameKeyInDeps(
     forall p :: p in b[i].environment.sentPackets && p.msg.Message_Read_Reply? ==> ReadReplyHasCorrspondingReadWithSmallerVC(b, i, p)
 }
 
-lemma lemma_BehaviorValidImpliesOneStepValid(
-    b:Behavior<CMState>,
-    i:int
-)
-    requires 0 < i
-    requires IsValidBehaviorPrefix(b, i)
-    ensures CMNext(b[i-1], b[i])
-{
-    ghost var j := i - 1;
-    assert 0 <= j < i;
-    assert j + 1 == i;
-    assert CMNext(b[j], b[j+1]);
-}
 
 lemma lemma_ReadReplyHasHigherVCThanDepsPrefix(
     b:Behavior<CMState>,
