IronFleetDefault/ironfleet/src/Dafny/Distributed/Protocol/CausalMesh/proof/read_after_write.dfy
@@ -1,0 +1,161 @@
+include "../distributed_system.dfy"
+include "causalcut.dfy"
+include "packet_sending.dfy"
+include "message_read_reply.dfy"
+include "../../../Common/Collections/Seqs.s.dfy"
+
+module CausalMesh_Proof_Read_After_Write_i {
+import opened CausalMesh_Cache_i
+import opened CausalMesh_Message_i
+import opened CausalMesh_Types_i
+import opened Environment_s
+import opened CausalMesh_DistributedSystem_i
+import opened CausalMesh_Properties_i
+import opened CausalMesh_Proof_Actions_i
+import opened Temporal__Temporal_s
+import opened CausalMesh_proof_Assumptions_i
+import opened CausalMesh_Proof_Constants_i
+import opened CausalMesh_Proof_CausalCut_i
+import opened CausalMesh_Proof_PacketSending_i
+import opened CausalMesh_Proof_MessageReadReply_i
+import opened Collections__Seqs_s
+import opened Collections__Maps_i
+import opened Collections__Maps2_s
+
+// lemma lemma_AllDepsInCCacheAfterPullDepsAreExistsInICache()
+
+predicate WriteReplyIsLargerThanVCInDeps(deps:Dependency, vc:VectorClock)
+    requires DependencyValid(deps)
+    requires VectorClockValid(vc)
+{
+    forall k :: k in deps ==> VCHappendsBefore(deps[k], vc) || VCEq(deps[k], vc)
+}
+
+predicate WriteReplyIsLargerThanVCInLocal(local:map<Key, Meta>, vc:VectorClock)
+    requires forall k :: k in local ==> MetaValid(local[k])
+    requires VectorClockValid(vc)
+{
+    forall k :: k in local ==> VCHappendsBefore(local[k].vc, vc) || VCEq(local[k].vc, vc)
+}
+
+predicate WriteReplyHasCorrspondingWriteWithSmallerVC(
+    b:Behavior<CMState>,
+    i:int,
+    p:Packet
+)
+    requires 0 < i 
+    requires IsValidBehaviorPrefix(b, i)
+    requires p in b[i].environment.sentPackets && p.msg.Message_Write_Reply? && PacketValid(p)
+{
+    lemma_BehaviorValidImpliesOneStepValid(b, i);
+    forall wp :: wp in b[i].environment.sentPackets && wp.msg.Message_Write?
+                    && p.msg.key_wreply == wp.msg.key_write
+                    && p.dst == wp.src
+                    ==> WriteReplyIsLargerThanVCInDeps(wp.msg.deps_write, p.msg.vc_wreply)
+                        && WriteReplyIsLargerThanVCInLocal(wp.msg.local, p.msg.vc_wreply)
+}
+
+predicate AllWriteReplyHasCoorspondingWriteWithSmallerOrEqVCInDepsAndLocals(
+    b:Behavior<CMState>,
+    i:int
+)
+    requires 0 < i 
+    requires IsValidBehaviorPrefix(b, i)
+{
+    lemma_BehaviorValidImpliesOneStepValid(b, i);
+
+    forall p :: p in b[i].environment.sentPackets && p.msg.Message_Write_Reply? ==> WriteReplyHasCorrspondingWriteWithSmallerVC(b, i, p)
+}
+
+predicate ReadReplyVCIsLargerThanAllPreviousWrites(
+    b:Behavior<CMState>,
+    i:int,
+    p:Packet
+)
+    requires 0 < i 
+    requires IsValidBehaviorPrefix(b, i)
+    requires p in b[i].environment.sentPackets && p.msg.Message_Read_Reply? && PacketValid(p)
+{
+    lemma_BehaviorValidImpliesOneStepValid(b, i);
+    forall wrp :: wrp in b[i].environment.sentPackets && wrp.msg.Message_Write_Reply?
+            && p.msg.key_rreply == wrp.msg.key_wreply
+            && (VCHappendsBefore(wrp.msg.vc_wreply, p.msg.vc_rreply) || VCEq(wrp.msg.vc_wreply, p.msg.vc_rreply))
+                ==> WriteReplyHasCorrspondingWriteWithSmallerVC(b, i, wrp)
+}
+
+lemma lemma_WriteReplyHasHigerVCThanDepsAndLocalPrefix(
+    b:Behavior<CMState>,
+    i:int
+)
+    requires 0 < i 
+    requires IsValidBehaviorPrefix(b, i)
+    requires forall j :: 0 <= j < i ==> CMNext(b[j], b[j+1])
+    // ensures AllWriteReplyHasCoorspondingWriteWithSmallerOrEqVCInDepsAndLocals(b, i)
+    decreases i
+{
+    if i <= i {
+        return;
+    }
+
+    lemma_ConstantsAllConsistent(b, i-1);
+    lemma_ConstantsAllConsistent(b, i);
+
+    if !StepSendsWriteReply(b[i-1], b[i]){
+        lemma_WriteReplyHasHigerVCThanDepsAndLocalPrefix(b, i-1);
+        return;
+    }
+
+    lemma_WriteReplyHasHigerVCThanDepsAndLocalPrefix(b, i-1);
+
+    var p :| p in b[i].environment.sentPackets && p !in b[i-1].environment.sentPackets && p.msg.Message_Write_Reply?;
+
+    assert PacketValid(p);
+
+    var idx, ios := lemma_ActionThatSendsWriteReplyIsServerReceiveWrite(b[i-1], b[i], p);
+
+    var p_write := ios[0].r;
+    var sp := ExtractSentPacketsFromIos(ios);
+
+    assert ReceiveWrite(b[i-1].servers[idx].s, b[i].servers[idx].s, p_write, sp);
+}
+
+predicate StepSendsWriteReply(s:CMState, s':CMState)
+    requires CMNext(s, s')
+{
+    // && s.environment.nextStep.LEnvStepHostIos?
+    && exists p :: p in s'.environment.sentPackets && p.msg.Message_Write_Reply? && p !in s.environment.sentPackets
+}
+
+lemma lemma_ServerWriteReplyLargerVCThanLocalAndDeps(s:Server, s':Server, p:Packet, sp:seq<Packet>)
+    requires p.msg.Message_Write?
+    requires ServerValid(s)
+    requires PacketValid(p) 
+    requires ReceiveWrite(s, s', p, sp)
+    ensures |sp| == 2
+    ensures sp[0].msg.Message_Write_Reply?
+    ensures forall k :: k in p.msg.local ==> 
+                VCHappendsBefore(p.msg.local[k].vc, sp[0].msg.vc_wreply) || VCEq(p.msg.local[k].vc, sp[0].msg.vc_wreply)
+    ensures forall k :: k in p.msg.deps_write ==> 
+                VCHappendsBefore(p.msg.deps_write[k], sp[0].msg.vc_wreply) || VCEq(p.msg.deps_write[k], sp[0].msg.vc_wreply)
+{
+    assert forall k :: k in p.msg.local ==> MetaValid(p.msg.local[k]);
+    var local_metas := set m | m in p.msg.local.Values;
+    var vcs_local := set m | m in local_metas :: m.vc;
+    assert forall vc :: vc in vcs_local ==> VectorClockValid(vc); 
+    var merged_vc := FoldVC(s.gvc, vcs_local);
+    assert forall vc :: vc in vcs_local ==> VCHappendsBefore(vc, merged_vc) || VCEq(vc, merged_vc);
+    assert forall m :: m in local_metas ==> VCHappendsBefore(m.vc, merged_vc) || VCEq(m.vc, merged_vc);
+    assert forall k :: k in p.msg.local ==> p.msg.local[k] in local_metas;
+    assert forall k :: k in p.msg.local ==> 
+                VCHappendsBefore(p.msg.local[k].vc, sp[0].msg.vc_wreply) || VCEq(p.msg.local[k].vc, sp[0].msg.vc_wreply);
+
+    var vcs_deps := set k | k in p.msg.deps_write :: p.msg.deps_write[k];
+    var merged_vc2 := FoldVC(merged_vc, vcs_deps);
+    assert forall vc :: vc in vcs_deps ==> VCHappendsBefore(vc, merged_vc2) || VCEq(vc, merged_vc2);
+    assert forall k :: k in p.msg.deps_write ==> 
+                VCHappendsBefore(p.msg.deps_write[k], merged_vc2) || VCEq(p.msg.deps_write[k], merged_vc2);
+    assert forall k :: k in p.msg.deps_write ==> 
+                VCHappendsBefore(p.msg.deps_write[k], sp[0].msg.vc_wreply) || VCEq(p.msg.deps_write[k], sp[0].msg.vc_wreply);
+}
+
+}
